slight modification of hole transition rule

lio.v
@@ -478,8 +478,8 @@ Inductive lio_reduce : m -> m -> Prop :=    (* defn lio_reduce *)
       n'' = n' +1  ->
      pure_reduce (t_CanFlowTo l' l1) t_VTrue ->
      lio_reduce (m_Config l_5 c (t_ToLabeled l1 t5) n5) (m_Config l_5 c (t_Label l1 t') n'')
- | LIO_hole : forall (n5:n),
-     lio_reduce (m_Config t_VHole t_VHole t_VHole n5) (m_Config t_VHole t_VHole t_VHole n5)
+ | LIO_hole : forall (t1 t2:t) (n5:n),
+     lio_reduce (m_Config t1 t2 t_VHole n5) (m_Config t1 t2 t_VHole n5)
 with lio_reduce_multi : m -> m -> Prop :=    (* defn lio_reduce_multi *)
  | LIO_onestep : forall (l5 c t5:t) (n5:n) (l' c' t':t) (n':n),
      is_l_of_t l5 ->
